first pass at typeclass sort eq

theories/Init/Types/Equality.v
@@ -27,40 +27,88 @@ Definition eqdiag@{s|l|} {A : Type@{s|l}} := eq@{s s| l} (A:=A).
 Notation "x ≡ y" := (eqdiag x y) (at level 60) : type_scope.
 Notation "x ≡ y :> A" := (@eqdiag A x y) (at level 60) : type_scope.
 
-Definition eq_ind@{s | u|} [A] [x] P := @eq_elim@{s Prop|u Set} A x (fun a _ => P a).
+#[projections(primitive=no)]
+Class hasJ@{s s' s''| u v | } :=
+{
+  J : forall [A : Type@{s|u}] [x : A]
+        (P : forall a : A, (eq@{s s'|u} x a) -> Type@{s''|v}),
+        P x eq_refl ->
+        forall (y : A) (e : eq@{_ s' | _} x y),
+        P y e;
 
-Definition eq_singleton@{s s' | u v|} [A:Type@{s|u}] [x:A]
+  J_refl : forall (A : Type@{s|u}) (x : A)
+              (P : forall a : A, (eq@{s s'|u} x a) -> Type@{s''|v})
+              (t : P x eq_refl),
+              eq@{_ s' | _} (J P t x eq_refl) t
+}.
+
+Register J as core.eq.poly.
+
+#[export]
+Instance hasJ_eqelim@{s s'|u v|} : hasJ@{s s' s'|u v} := {
+  J := eq_elim@{s s'|u v};
+  J_refl := fun A x P t => eq_refl
+}.
+
+#[export]
+Instance hasJ_Type@{s s'|u v|} : hasJ@{s Type s'|u v} := {
+  J := fun A x P t y e => match e with eq_refl => t end;
+  J_refl := fun A x P t => eq_refl
+}.
+
+Definition J_nodep@{s s' s''| u  v|} `{hasJ@{s s' s''| u v}} [A:Type@{s|u}] [x:A]
+  (P : A -> Type@{s''|v}) : P x -> forall (y:A) (e: eq@{_ s' | _} x y), P y  := J (fun y _ => P y).
+
+(* Register J_nodep as core.eq.eq_poly. *)
+Register J_nodep as core.eq.ind.
+
+(* Definition eq_ind@{s|u|} `{hasJ@{s Prop Prop|u Set}} := J_nodep.
+Register eq_ind as core.eq.ind. *)
+
+
+(* Are these actually useful? (besides providing a name) *)
+(* Instance eq_ind@{s|u|} : hasJ@{s Prop|u Set} := hasJ_eqelim@{s Prop| u Set}.
+Instance eq_nodep_ind@{s|u|} `{hasJ@{s Prop| u Set}} : hasNoDepJ := hasNoDepJ_from_hasJ. *)
+
+
+(* Definition eq_ind@{s | u|} [A] [x] P := @eq_elim@{s Prop|u Set} A x (fun a _ => P a). *)
+
+(* Instance eq_singleton@{s | u v|} : hasJ@{s Prop | u v} := hasJ_eqelim@{s Prop| u v}. *)
+(* Definition eq_singleton@{s s' | u v|} [A:Type@{s|u}] [x:A]
   (P : forall a : A, (eq@{s Prop|u} x a) -> Type@{s'|v}) :
   P x (eq_refl x) -> forall [a : A] (e : x = a :> A), P a e :=
-  fun t _ e => match e with eq_refl => t end.
+  fun t _ e => match e with eq_refl => t end. *)
 
-Definition eq_rect@{u v|} [A:Type@{u}] [x:A]
+
+(* Instance eq_nodep_rect@{u v|} `{hasJ@{Type Type | u v}} : hasNoDepJ := hasNoDepJ_from_hasJ@{Type Type| u v}. *)
+
+(* Definition eq_rect@{u v|} [A:Type@{u}] [x:A]
   (P : forall a : A, Type@{v}) :
-  P x -> forall [a : A] (e : x = a :> A), P a := @eq_singleton A x (fun a _ => P a).
+  P x -> forall [a : A] (e : x = a :> A), P a := @eq_singleton A x (fun a _ => P a). *)
 
-Definition eq_rec@{u|} [A:Type@{u}] [x:A]
+(* Definition eq_rec@{u|} [A:Type@{u}] [x:A]
   (P : forall a : A, Set) :
-  P x -> forall [a : A] (e : x = a :> A), P a := @eq_singleton A x (fun a _ => P a).
+  P x -> forall [a : A] (e : x = a :> A), P a := @eq_singleton A x (fun a _ => P a). *)
 
-Definition eq_sind [A:Set] [x:A]
+(* Definition eq_sind [A:Set] [x:A]
   (P : forall a : A, SProp) :
-  P x -> forall [a : A] (e : x = a :> A), P a := @eq_singleton A x (fun a _ => P a).
+  P x -> forall [a : A] (e : x = a :> A), P a := @eq_singleton A x (fun a _ => P a). *)
 
-Arguments eq_ind [A] x P _ y _ : rename.
+(* Arguments eq_ind [A] x P _ y _ : rename.
 Arguments eq_sind [A] x P _ y _ : rename.
 Arguments eq_rec [A] x P _ y _ : rename.
-Arguments eq_rect [A] x P _ y _ : rename.
+Arguments eq_rect [A] x P _ y _ : rename. *)
 
 Notation "x = y" := (eq@{_ Prop|_} x y) : type_scope.
 Notation "x <> y  :> T" := (~ x = y :>T) : type_scope.
 Notation "x <> y" := (~ (x = y)) : type_scope.
 
-#[global]
+#[export]
 Hint Resolve eq_refl: core.
 
 Section GroupoidOperations.
   Sort sa se.
-  Universe a.
+  Universes a.
   Context {A : Type@{sa|a}}.
   #[warnings="-notation-overridden"]
   Local Notation "x = y" := (eq@{_ se|_} x y) : type_scope.
@@ -70,13 +118,13 @@ Section GroupoidOperations.
 
 (** listings: eqtrans **)
 Definition eq_trans {x y z : A} (e1 : x = y) : y = z -> x = z :=
-    match e1 with | eq_refl _ => fun x => x end.
+  match e1 with | eq_refl _ => fun x => x end.
 (** listings: end **)
 
   Definition tr@{b|} {B : Type@{sa|b}} (e : @eq@{_ sa|max(a+1,b+1)} Type@{sa|max(a,b)} A B) : A -> B :=
     match e in @eq _ _ B return A -> B with | eq_refl _ => fun x => x end.
 
-  Definition ap@{sb|b|} {B : Type@{sb|b}} (f : A -> B) {x y : A} (e : x = y) : f x = f y :=
+  Definition ap@{sb|b|} {B : Type@{sb|b}} (f : A -> B) {x y : A} (e : eq@{_ se|_} x y) : eq@{_ se|_} (f x) (f y) :=
     match e with | eq_refl _ => eq_refl _ end.
 
 End GroupoidOperations.
@@ -84,67 +132,75 @@ Notation congr := ap.
 
 Register eq as core.eq.type.
 Register eq_refl as core.eq.refl.
-Register eq_ind as core.eq.ind.
+(* Register eq_ind as core.eq.ind.
 Register eq_rect as core.eq.rect.
-Register eq_elim as core.eq.rect.
+Register eq_elim as core.eq.rect. *)
 Register eq_sym as core.eq.sym.
 Register eq_trans as core.eq.trans.
 Register congr as core.eq.congr.
 
-Definition eq_elim_r@{α β|u v|} (A:Type@{α|u}) (x:A) (P:A -> Type@{β|v}) :
-  P x -> forall y:A, eq@{_ β | _} y x -> P y :=
-  fun px y e =>
-    match e in _ = x return P x -> P y with
-    | eq_refl => fun py => py
-    end px.
+Definition J_nodep_r@{s s' s''|u v|} `{hasJ@{s s' s''|u v}}
+  (A:Type@{s|u}) (x:A)
+  (P:A -> Type@{s''|v}) (t : P x)
+  (y:A) (e : eq@{s s' | u} y x) : P y :=
+  J_nodep P t y (eq_sym e).
 
-Register eq_elim_r as core.eq.poly_r.
+Register J_nodep_r as core.eq.poly_r.
+Register J_nodep_r as core.eq.eq_rect_r.
+(* Register J_nodep_r as core.eq.ind. *)
+Register J_nodep_r as core.eq.ind_r.
 
-Definition eq_rect_r@{α β|u v|} (A:Type@{α|u}) (x:A) (P:A -> Type@{β|v}) :
+(* Definition eq_rect_r@{s s'|u v|} `{hasJ@{s Type s'|u v}} := eq_elim_r. *)
+
+(* Definition eq_rect_r@{α β|u v|} (A:Type@{α|u}) (x:A) (P:A -> Type@{β|v}) :
   P x -> forall y:A, eq@{α Type|_} y x -> P y :=
   fun px y e =>
   match e in _ = x return P x -> P y with
   | eq_refl => fun py => py
-  end px.
+  end px. *)
 
-Register eq_rect_r as core.eq.rect_r.
+(* Register eq_rect_r as core.eq.rect_r.  *)
 
-Definition eq_singleton_r@{α β|u v|} (A:Type@{α|u}) (x:A) (P:A -> Type@{β|v}) :
+(* Same as eq_elim_r ? *)
+(* Definition eq_singleton_r@{α β|u v|} (A:Type@{α|u}) (x:A) (P:A -> Type@{β|v}) :
   P x -> forall y:A, y = x -> P y :=
   fun px y e =>
     match e in _ = x return P x -> P y with
     | eq_refl => fun py => py
-    end px.
+    end px. *)
 
-Definition eq_ind_r@{α|u|} := eq_singleton_r@{α Prop | u Set}.
+(* Definition eq_ind_r@{s|u|} `{hasJ@{s Prop Prop| u Set}} := eq_elim_r. *)
 
-Register eq_ind_r as core.eq.ind_r.
+(* Register eq_ind_r as core.eq.ind_r. *)
+(* Register eq_ind_r as core.eq.ind. *)
 
-Definition eq_elim_d@{α β|u v|} (A:Type@{α|u}) (x:A) (P:A -> Type@{β|v}) :
+(* Same as eq_elim_r? *)
+(* Definition eq_elim_d@{α β|u v|} (A:Type@{α|u}) (x:A) (P:A -> Type@{β|v}) :
   P x -> forall y:A, eq@{_ β |_} x y -> P y :=
   fun px y e =>
     match e in _ = y return P x -> P y with
     | eq_refl => fun px => px
     end px.
 
-Register eq_elim_d as core.eq.poly.
+Register eq_elim_d as core.eq.poly. *)
 
-Definition eq_rect_d@{α β|u v|} (A:Type@{α|u}) (x:A) (P:A -> Type@{β|v}) :
+(* Definition eq_rect_d@{α β|u v|} (A:Type@{α|u}) (x:A) (P:A -> Type@{β|v}) :
   P x -> forall y:A, eq@{α Type|_} x y -> P y :=
   fun px y e =>
   match e in _ = y return P x -> P y with
   | eq_refl => fun py => py
   end px.
 
-Register eq_rect_d as core.eq.rect.
+Register eq_rect_d as core.eq.rect. *)
 
-Definition eq_ind_d@{α β|u v|} (A:Type@{α|u}) (x:A) (P:A -> Type@{β|v}) :
+(* Definition eq_ind_d@{α β|u v|} (A:Type@{α|u}) (x:A) (P:A -> Type@{β|v}) :
   P x -> forall y:A, x = y -> P y := eq_singleton (fun y _ => P y).
 
-Register eq_ind_d as core.eq.ind.
+Register eq_ind_d as core.eq.ind. *)
 
 Definition f_equal@{s s' e|u v|} {A : Type@{s|u}} {B : Type@{s'|v}} (f : A -> B) {x y} : eq@{_ e| _} x y -> eq@{_ e| _} (f x) (f y) :=
   fun e => match e with | eq_refl => eq_refl end.
+  (* @ap@{s s' e|u v} A B f x y. *)
 
 Register f_equal as core.eq.congr.
 
