theories/Tactics/Equality.v
@@ -1,0 +1,14 @@
+(* These should go in their own file *)
+From Ltac2 Require Import Ltac2.
+
+Ltac2 rewrite0 (h : constr) :=
+    unshelve (eapply (J_nodep _ _ _ _ _ $h)).
+
+#[global]
+Ltac2 Notation "rewrite!" h(constr) := rewrite0 h.
+
+Ltac2 rewrite0_r (h : constr) :=
+  unshelve (eapply (J_nodep_r _ _ _ _ _ (eq_sym $h))).
+
+#[global]
+Ltac2 Notation "rewrite!" "<-" h(constr) := rewrite0_r h.
